Weidenbach_Book/IsaSAT_Rephase_LLVM.thy
@@ -1,5 +1,5 @@
 theory IsaSAT_Rephase_LLVM
-  imports IsaSAT_Rephase IsaSAT_Setup_LLVM
+  imports IsaSAT_Rephase IsaSAT_Show_LLVM
 begin
 
 sepref_def rephase_random_impl
@@ -36,14 +36,16 @@ sepref_register rephase_init rephase_random copy_phase
 
 sepref_def phase_save_phase_impl
   is \<open>uncurry phase_save_phase\<close>
-  :: \<open>uint32_nat_assn\<^sup>k *\<^sub>a phase_heur_assn\<^sup>d \<rightarrow>\<^sub>a phase_heur_assn\<close>
+  :: \<open>sint64_nat_assn\<^sup>k *\<^sub>a phase_heur_assn\<^sup>d \<rightarrow>\<^sub>a phase_heur_assn\<close>
+  supply [[goals_limit=1]]
   unfolding phase_save_phase_def
   by sepref
 
 
 sepref_def save_phase_heur_impl
   is \<open>uncurry save_rephase_heur\<close>
-  ::  \<open>uint32_nat_assn\<^sup>k *\<^sub>a heuristic_assn\<^sup>d \<rightarrow>\<^sub>a heuristic_assn\<close>
+  ::  \<open>sint64_nat_assn\<^sup>k *\<^sub>a heuristic_assn\<^sup>d \<rightarrow>\<^sub>a heuristic_assn\<close>
+  supply [[goals_limit=1]]
   unfolding save_rephase_heur_def heuristic_assn_def
   by sepref
 
@@ -51,6 +53,7 @@ sepref_def save_phase_heur_impl
 sepref_def save_phase_heur_st
   is save_phase_st
   ::  \<open>isasat_bounded_assn\<^sup>d \<rightarrow>\<^sub>a isasat_bounded_assn\<close>
+  supply [[goals_limit=1]]
   unfolding save_phase_st_def isasat_bounded_assn_def
   by sepref
 
@@ -67,12 +70,26 @@ sepref_def rephase_heur_impl
   unfolding rephase_heur_def heuristic_assn_def
   by sepref
 
+lemma current_rephasing_phase_alt_def:
+  \<open>RETURN o current_rephasing_phase =
+    (\<lambda>(fast_ema, slow_ema, res_info, wasted, (\<phi>, target_assigned, target, best_assigned, best, end_of_phase, curr_phase, length_phase)).   RETURN curr_phase)\<close>
+  unfolding current_rephasing_phase_def
+    phase_current_rephasing_phase_def
+  by (auto intro!: ext)
+
+sepref_def current_rephasing_phase
+  is \<open>RETURN o current_rephasing_phase\<close>
+  :: \<open>heuristic_assn\<^sup>k \<rightarrow>\<^sub>a word_assn\<close>
+  unfolding current_rephasing_phase_alt_def heuristic_assn_def
+  by sepref
 
 sepref_def rephase_heur_st_impl
   is rephase_heur_st
   ::  \<open>isasat_bounded_assn\<^sup>d \<rightarrow>\<^sub>a isasat_bounded_assn\<close>
   unfolding rephase_heur_st_def isasat_bounded_assn_def
   by sepref
+
+term current_rephasing_phase
 
 experiment
 begin
@@ -81,3 +98,4 @@ export_llvm rephase_heur_st_impl
 end
 
 end
+
