Weidenbach_Book/IsaSAT_Setup_LLVM.thy
@@ -76,10 +76,10 @@ lemmas [llvm_inline] =
   incr_GC_def
 
 
-abbreviation (input) "restart_info_rel \<equiv> word64_rel \<times>\<^sub>r word64_rel \<times>\<^sub>r word64_rel \<times>\<^sub>r word64_rel"
+abbreviation (input) "restart_info_rel \<equiv> word64_rel \<times>\<^sub>r word64_rel \<times>\<^sub>r word64_rel \<times>\<^sub>r word64_rel \<times>\<^sub>r word64_rel"
 
 abbreviation (input) restart_info_assn where
-  \<open>restart_info_assn \<equiv> word64_assn *a word64_assn *a word64_assn *a word64_assn\<close>
+  \<open>restart_info_assn \<equiv> word64_assn *a word64_assn *a word64_assn *a word64_assn *a word64_assn\<close>
 
 lemma restart_info_params[sepref_import_param]:
   "(incr_conflict_count_since_last_restart,incr_conflict_count_since_last_restart) \<in>
@@ -226,7 +226,7 @@ abbreviation phase_saver_assn :: \<open>phase_saver \<Rightarrow> phase_saver_as
 (* TODO: Move *)
 type_synonym arena_assn = "(32 word, 64) array_list"
 type_synonym heur_assn = \<open>(ema \<times> ema \<times> restart_info \<times> 64 word \<times>
-   phase_saver_assn \<times> 32 word \<times> phase_saver_assn \<times> 32 word \<times> phase_saver_assn \<times> 64 word \<times> 64 word \<times> 64 word)\<close>
+   phase_saver_assn \<times> 64 word \<times> phase_saver_assn \<times> 64 word \<times> phase_saver_assn \<times> 64 word \<times> 64 word \<times> 64 word)\<close>
 
 type_synonym twl_st_wll_trail_fast =
   \<open>trail_pol_fast_assn \<times> arena_assn \<times> option_lookup_clause_assn \<times>
@@ -237,9 +237,9 @@ type_synonym twl_st_wll_trail_fast =
 
 
 abbreviation phase_heur_assn where
-  \<open>phase_heur_assn \<equiv> phase_saver_assn *a uint32_nat_assn *a phase_saver_assn *a uint32_nat_assn *a
+  \<open>phase_heur_assn \<equiv> phase_saver_assn *a sint64_nat_assn *a phase_saver_assn *a sint64_nat_assn *a
      phase_saver_assn *a word64_assn *a word64_assn *a word64_assn\<close>
-     
+
 definition heuristic_assn :: \<open>restart_heuristics \<Rightarrow> heur_assn \<Rightarrow> assn\<close> where
   \<open>heuristic_assn = ema_assn *a
   ema_assn *a
