Weidenbach_Book/IsaSAT_Show_LLVM.thy
@@ -4,18 +4,8 @@ theory IsaSAT_Show_LLVM
     IsaSAT_Setup_LLVM
 begin
 
-text \<open>The printing has been removed.\<close>
-lemma isasat_current_information_alt_def:
-\<open>isasat_current_information =
-   (\<lambda>(propa, confl, decs, frestarts, lrestarts, uset, gcs, lbds) lcount.
-     if confl AND 8191 = 8191 \<comment> \<open>\<^term>\<open>8191 = 8192 - 1\<close>, i.e., we print when all first bits are 1.\<close>
-     then
-        zero_some_stats (propa, confl, decs, frestarts, lrestarts, uset, gcs, lbds)
-      else (propa, confl, decs, frestarts, lrestarts, uset, gcs, lbds)
-      )\<close>
-  unfolding isasat_current_information_def by auto
 
-sepref_register print_current_information print_c print_uint64
+sepref_register isasat_current_information print_c print_uint64
 
 sepref_def print_c_impl
   is \<open>RETURN o print_c\<close>
@@ -29,6 +19,24 @@ sepref_def print_uint64_impl
   unfolding print_uint64_def
   by sepref
 
+sepref_def print_open_colour_impl
+  is \<open>RETURN o print_open_colour\<close>
+  :: \<open>word_assn\<^sup>k \<rightarrow>\<^sub>a unit_assn\<close>
+  unfolding print_open_colour_def
+  by sepref
+
+
+sepref_def print_close_colour_impl
+  is \<open>RETURN o print_close_colour\<close>
+  :: \<open>word_assn\<^sup>k \<rightarrow>\<^sub>a unit_assn\<close>
+  unfolding print_close_colour_def
+  by sepref
+
+sepref_def print_char_impl
+  is \<open>RETURN o print_char\<close>
+  :: \<open>word_assn\<^sup>k \<rightarrow>\<^sub>a unit_assn\<close>
+  unfolding print_char_def
+  by sepref
 
 sepref_def zero_some_stats_impl
   is \<open>RETURN o zero_some_stats\<close>
@@ -37,9 +45,9 @@ sepref_def zero_some_stats_impl
   by sepref
 
 sepref_def isasat_current_information_impl [llvm_code]
-  is \<open>uncurry (RETURN oo print_current_information)\<close>
-  :: \<open>stats_assn\<^sup>k *\<^sub>a uint64_nat_assn\<^sup>k \<rightarrow>\<^sub>a stats_assn\<close>
-  unfolding print_current_information_isasat_current
+  is \<open>uncurry2 (RETURN ooo isasat_current_information)\<close>
+  :: \<open>word_assn\<^sup>k *\<^sub>a stats_assn\<^sup>k *\<^sub>a uint64_nat_assn\<^sup>k \<rightarrow>\<^sub>a stats_assn\<close>
+  unfolding isasat_current_information_def
     isasat_current_information_def
   by sepref
 
@@ -63,26 +71,6 @@ sepref_def isasat_current_status_fast_code
   supply [[goals_limit=1]]
   unfolding isasat_bounded_assn_def isasat_current_status_def
   unfolding fold_tuple_optimizations
-  by sepref
-
-
-sepref_def print_open_colour_impl
-  is \<open>RETURN o print_open_colour\<close>
-  :: \<open>word_assn\<^sup>k \<rightarrow>\<^sub>a unit_assn\<close>
-  unfolding print_open_colour_def
-  by sepref
-
-
-sepref_def print_close_colour_impl
-  is \<open>RETURN o print_close_colour\<close>
-  :: \<open>word_assn\<^sup>k \<rightarrow>\<^sub>a unit_assn\<close>
-  unfolding print_close_colour_def
-  by sepref
-
-sepref_def print_char_impl
-  is \<open>RETURN o print_char\<close>
-  :: \<open>word_assn\<^sup>k \<rightarrow>\<^sub>a unit_assn\<close>
-  unfolding print_char_def
   by sepref
 
 sepref_def isasat_print_progress_impl
